src/QUIC.Secret.Buffer.fst
@@ -1,0 +1,39 @@
+module QUIC.Secret.Buffer
+
+friend Lib.IntTypes
+
+module Secret = QUIC.Secret.Int
+module B = LowStar.Buffer
+module U8 = FStar.UInt8
+module HS = FStar.HyperStack
+module HST = FStar.HyperStack.ST
+module Seq = QUIC.Secret.Seq
+module Ghost = FStar.Ghost
+
+#set-options "--z3rlimit 64" // --query_stats"
+
+#restart-solver
+
+let seq_hide_eq
+  (#t: Secret.inttype { Secret.unsigned t })
+  (#sec: Secret.secrecy_level)
+  (x: Seq.seq (Secret.uint_t t sec))
+: Lemma
+  (Seq.seq_hide x `Seq.equal` x)
+  [SMTPat (Seq.seq_hide x)]
+= ()
+
+let seq_reveal_eq
+  (#t: Secret.inttype { Secret.unsigned t })
+  (#sec: Secret.secrecy_level)
+  (x: Seq.seq (Secret.uint_t t sec))
+: Lemma
+  (Seq.seq_reveal x `Seq.equal` x)
+  [SMTPat (Seq.seq_reveal x)]
+= ()
+
+let with_buffer_hide #t b from to h0 lin lout x1 x2 x3 x4 x5 x6 post f =
+  let bl = B.sub b 0ul from in
+  let bs = B.sub b from (to `U32.sub` from) in
+  let br = B.offset b to in
+  f (Ghost.hide (B.loc_buffer b)) bl bs br
