src/QUIC.Secret.Buffer.fsti
@@ -1,0 +1,61 @@
+module QUIC.Secret.Buffer
+
+module Secret = QUIC.Secret.Int
+module B = LowStar.Buffer
+module U8 = FStar.UInt8
+module HS = FStar.HyperStack
+module HST = FStar.HyperStack.ST
+module Seq = QUIC.Secret.Seq
+module Ghost = FStar.Ghost
+
+module U32 = FStar.UInt32
+
+#set-options "--z3rlimit 16"
+
+inline_for_extraction
+noextract
+val with_buffer_hide
+  (#t: Type)
+  (b: B.buffer U8.t)
+  (from: U32.t)
+  (to: U32.t { U32.v from <= U32.v to /\ U32.v to <= B.length b })
+  (h0: HS.mem)
+  (lin: Ghost.erased B.loc { B.loc_disjoint (Ghost.reveal lin) (B.loc_buffer b) })
+  (lout: Ghost.erased B.loc { B.loc_disjoint (Ghost.reveal lout) (B.loc_buffer b) })
+  (x1 x2 x3 x4 x5: Ghost.erased U32.t)
+  (x6: Ghost.erased U32.t {
+    U32.v x1 <= U32.v x2 /\ U32.v x2 <= U32.v from /\
+    U32.v x3 <= U32.v x4 /\ U32.v x4 <= U32.v to - U32.v from /\
+    U32.v x5 <= U32.v x6 /\ U32.v x6 <= B.length b - U32.v to
+  })
+  (post: (res: t) ->  (contl: Seq.lseq U8.t (U32.v from)) ->  (cont: Seq.lseq U8.t (U32.v to - U32.v from)) ->  (contr: Seq.lseq U8.t (B.length b - U32.v to)) -> (h: HS.mem) -> GTot Type0)
+  (f: (
+    (l: Ghost.erased B.loc) ->
+    (bl: B.buffer U8.t { B.length bl == (U32.v from) }) ->
+    (bs: B.buffer Secret.uint8 { B.length bs == (U32.v to - U32.v from) }) ->
+    (br: B.buffer U8.t { B.length br == (B.length b - U32.v to) }) ->
+    HST.Stack t
+    (requires (fun h ->
+      B.modifies l h0 h /\
+      B.loc_disjoint (B.loc_buffer bl `B.loc_union` B.loc_buffer bs) (B.loc_buffer br) /\
+      B.loc_disjoint (B.loc_buffer bl) (B.loc_buffer bs) /\
+      B.loc_disjoint (Ghost.reveal lin `B.loc_union` Ghost.reveal lout) (Ghost.reveal l `B.loc_union` B.loc_buffer bl `B.loc_union` B.loc_buffer bs `B.loc_union` B.loc_buffer br) /\
+      B.live h bl /\ B.live h bs /\ B.live h br /\
+      B.as_seq h bl == B.as_seq h0 (B.gsub b 0ul from) /\
+      Seq.seq_reveal (B.as_seq h bs) == B.as_seq h0 (B.gsub b from (to `U32.sub` from)) /\
+      B.as_seq h br == B.as_seq h0 (B.gsub b to (B.len b `U32.sub` to))
+    ))
+    (ensures (fun h res h' ->
+      B.modifies (Ghost.reveal lout `B.loc_union` (if U32.v x1 = U32.v x2 then B.loc_none else B.loc_buffer (B.gsub bl x1 (x2 `U32.sub` x1))) `B.loc_union` (if U32.v x3 = U32.v x4 then B.loc_none else B.loc_buffer (B.gsub bs x3 (x4 `U32.sub` x3))) `B.loc_union` (if U32.v x5 = U32.v x6 then B.loc_none else B.loc_buffer (B.gsub br x5 (x6 `U32.sub` x5)))) h h' /\
+      post res (B.as_seq h' bl) (Seq.seq_reveal (B.as_seq h' bs)) (B.as_seq h' br) h'
+    ))
+  ))
+: HST.Stack t
+  (requires (fun h ->
+    B.live h b /\
+    h0 == h
+  ))
+  (ensures (fun h res h' ->
+    B.modifies (Ghost.reveal lout `B.loc_union` (if U32.v x1 = U32.v x2 then B.loc_none else B.loc_buffer (B.gsub b x1 (x2 `U32.sub` x1))) `B.loc_union` (if U32.v x3 = U32.v x4 then B.loc_none else B.loc_buffer (B.gsub b (from `U32.add` x3) (x4 `U32.sub` x3))) `B.loc_union` (if U32.v x5 = U32.v x6 then B.loc_none else B.loc_buffer (B.gsub b (to `U32.add` x5) (x6 `U32.sub` x5)))) h h' /\
+    post res (B.as_seq h' (B.gsub b 0ul from)) (B.as_seq h' (B.gsub b from (to `U32.sub` from))) (B.as_seq h' (B.gsub b to (B.len b `U32.sub` to))) h'
+  ))
